src/RawAst/Types.dfy
@@ -7,29 +7,4 @@ module Types {
   const IntTypeName := "int"
   const TagTypeName := "tag"
   const BuiltInTypes: set<TypeName> := {BoolTypeName, IntTypeName, TagTypeName}
-
-  datatype Type =
-    | BoolType
-    | IntType
-    | TagType
-    | UserType(decl: TypeDecl)
-  {
-    function ToString(): string {
-      match this
-      case BoolType => BoolTypeName
-      case IntType => IntTypeName
-      case TagType => TagTypeName
-      case UserType(decl) => decl.Name
-    }
-  }
-
-  class TypeDecl {
-    const Name: string
-    
-    constructor (name: string)
-      ensures Name == name
-    {
-      Name := name;
-    }
-  }
 }
